\input{preambula.tex}
\begin{document}
	\section*{1}
	\subsection*{a)}
	$$J_{f,a}=\begin{pmatrix}
		2x & -21y^2\\
		y^2-2 & 2xy\\
		1 & 1
	\end{pmatrix}(-1, 3) = \begin{pmatrix}
	-2 & -21\cdot9\\
	7 & -6\\
	1 & 1
	\end{pmatrix}$$
	\subsection*{b)}
	$$J_{f,a}=\begin{pmatrix}
		-\cos{(xy^2)}y^2 & -\cos{(xy^2)}2xy & 1\\
		-7 & 2e^{2y+z} & e^{2y+z}
	\end{pmatrix}(1, 2, -1)= \begin{pmatrix}
	-4\cos{4} & -4\cos{4} & 1 \\
	-7 & 2e^3 & e^3
	\end{pmatrix}$$
	\subsection*{c)}
	$$J_{f,a}=\begin{pmatrix}
		-\frac{xz}{(x^2+y^2+1)^2 } & 	-\frac{2yz}{(x^2+y^2+1)^2 } & 	\frac{1}{(x^2+y^2+1)^2 }  
	\end{pmatrix}(1,-1, 2) = \begin{pmatrix}
	-\frac49 & \frac49 & \frac19
	\end{pmatrix}$$
	\subsection*{d)}
	$$J_{f,a}= \begin{pmatrix}
		3x^2 \\
		2^x\cdot\ln2 \\
		\sin{x}
	\end{pmatrix}(\frac{\pi}{6}) = \begin{pmatrix}
	\frac{\pi^2}{12} \\
	2^{\frac{\pi}{6}}\cdot\ln2 \\
	\frac12
	\end{pmatrix}$$
	\section*{e)}
	$$J_{f,a} = \frac{2x}{1+x^4}(-1) = -1$$
	\section*{2}
	$$J_{f,a} = \begin{pmatrix}
		3 & 2y & 0 \\
		2x & 0 & 1
	\end{pmatrix}$$
	$$J_{g,a} = \begin{pmatrix}
		v & u \\
		-2 & 1 \\
		1 & 2v
	\end{pmatrix}$$
	$$J_{g,f(a)}\cdot J_{f,a} = \begin{pmatrix}
		x^2+2 & 3x+y^2\\
		-2 & 1 \\
		1 & 2x^2+2z
	\end{pmatrix}\cdot \begin{pmatrix}
	3 & 2y & 0\\
	2x & 0 & 1
	\end{pmatrix}= \begin{pmatrix}
		9x^2+3z+2xy^2 & 2x^2y & 3x+y^2\\
		-6+2x & -4y & 1 \\
		3+4x^3+4x & 2y & 2x^2+2z
	\end{pmatrix} $$
	$$J_{f\circ g,a} = \begin{pmatrix}
		9x^2+3z+2xy^2 & 2x^2y & 3x+y^2\\
		-6+2x & -4y & 1 \\
		3+4x^3+4x & 2y & 2x^2+2z
	\end{pmatrix}$$
	Матрицы равны. 
	\section*{3}
	$$J_{f,a} = \begin{pmatrix}
		y\cdot e^{xy} & x\cdot e^{xy} + 3
	\end{pmatrix}$$
		$$J_{g,a} = \begin{pmatrix}
		2x-y & -x
	\end{pmatrix}$$
	$$\begin{pmatrix}
		y\cdot e^{xy} & x\cdot e^{xy} + 3
	\end{pmatrix}\cdot(x^2-xy) + (e^{xy}+3y)\cdot\begin{pmatrix}
	2x-y & -x
	\end{pmatrix} = \begin{pmatrix}
	2xe^{xy}+x^2ye^{xy}-xy^2e^{xy}+6xy-3y^2 \\
	x^3e^{xy}-xe^{xy}-x^2ye^{xy}-6xy+3x^2
	\end{pmatrix}$$
	$$J_{f\cdot g, a} = \begin{pmatrix}
		(e^{xy}_3y)(x^2-xy)'_{x} & (e^{xy}_3y)(x^2-xy)'_{y}
	\end{pmatrix}  = \begin{pmatrix}
	2xe^{xy}+x^2ye^{xy}-xy^2e^{xy}+6xy-3y^2 \\
	x^3e^{xy}-xe^{xy}-x^2ye^{xy}-6xy+3x^2
	\end{pmatrix}$$
	Матрицы равны. 
	\section*{4}
	\subsection*{a)}
	$$\frac{\partial f}{\partial x}(0,0) = \lim_{\delta \to 0} =\frac{f(\delta , 0) - f(0,0 )}{\delta } = \frac{\sqrt[3]{\delta0}- 0 }{\delta} = 0$$
	$$\frac{\partial f} {\partial y}(0,0) = \lim_{\delta \to 0} =\frac{f(0, ) - f(0,0 )}{\delta } = \frac{\sqrt[3]{\delta0}- 0 }{\delta} = 0$$
		\subsection*{b)}
		Пусть $f$ дифференцируема в $(0, 0)$.  Тогда она имеет вид. 
	$$f(h_1,h_2) = 0 + 0 + 0 + \alpha\left((0,0), (h_1,h_2)\right)\sqrt{h_1^2 + h_2^2}$$
	$$\alpha = \frac{f}{\sqrt{h_1^2 + h_2^2}}$$
	$$\lim\limits_{(h_1,h_2)\to 0} \alpha = 0$$ Это означает что функция дифференцируема в точке (0, 0)
	
\end{document}