\input{preambula.tex}
\renewcommand{\t}{\frac{\sqrt2}{2}}
\begin{document}
	\section*{1}
	$$J_k = \int\frac{1}{(y^2+\alpha^2)^k}\d{dy} = \begin{bmatrix}g(y)  =\frac{1}{(y^2+\alpha^2)^k}\\
		f(y) = 1 \\
		F(y) = y \\
		g^{'}(y)  = \frac{-2ky}{(y^2+\alpha^2)^{k+1}}\end{bmatrix} = \frac{y}{(y^2+\alpha^2)^k} +2k\cdot\int\frac{y^2\text{\textpm} a^2}{(y^2+\alpha^2)^{k+1}}\d{dy} = $$
		$$  =\frac{y}{(y^2+\alpha^2)^k} + 2k\cdot J_k - 2k\alpha^2J_{k+1}	$$ 
		$$J_{k+1} = \frac{1}{2k\alpha^2}\left(\frac{y}{(y^2+\alpha^2)^k} + (2n-1)\cdot J_n\right)$$
		\section*{2)}
		\subsection*{a)} 
		$$\int \frac{x^4}{(x+1)^3}\dx = \int x-3 + \frac{6}{x+1} +\frac{-4}{(x+1)^2} + \frac{1}{(x+1)^3}\dx = \frac{x^2}{2} -3x + 6J_1 - 4J_2 + J_3  $$
		$$J_3 = \frac14\cdot \frac{x}{(x+1)^2} + \frac34\cdot J_2$$
		$$J_2 = \frac12\cdot\frac{x}{x+1} + \frac12J_1$$
	$$J_1 = \ln\|x+1\|$$		
	$$\int \frac{x^4}{(x+1)^3}\dx = -\frac{x^4}{2(x+1)^2} + x^2-4x + 6\ln\|x+1\| + \frac{2}{x+1} + C$$
	\subsection*{b)}
	$$\int\frac{1}{x^4+1}\dx$$ 
	$$x^4+1 = (x-\t+\t i)(x-\t -\t i)(x+\t-\t i)(x+\t+\t i) = (x^2+\sqrt2 x +1)(x^2-\sqrt2 x + 1)$$
	$$\frac{Ax+C}{(x^2+\sqrt2 x +1) } + \frac{Bx+D}{(x^2-\sqrt2 x +1) }  = \frac{1}{(x^2+\sqrt2 x +1)(x^2-\sqrt2 x + 1)}$$
	$$\begin{cases}1 = D-C\\
	0  =-A -\sqrt2 C + B -\sqrt2 B\\
	0 = -\sqrt2A-C+\sqrt{2}B - D\\
	0 = B-A\end{cases}\to \begin{cases}A = \frac{1}{2\sqrt2}\\
	C = -\frac12\\
	B = \frac{1}{2\sqrt2}\\
	D = \frac12\end{cases}$$ 
	$$\int\frac{1}{x^4+1}\dx = \int -\frac{\frac{x}{2\sqrt2}-\frac12}{x^2-\sqrt2x+1} +\frac{\frac{x}{2\sqrt2}+\frac12}{x^2+\sqrt2x+1}\dx =$$ $$\frac{1}{4\sqrt2}\left(-\ln(x^2-\sqrt2x+1) + \ln(x^2+\sqrt2x+1)-2\arctg(1-\sqrt2x) + \arctg(\sqrt2x+1)\right) + C$$
	\subsection*{d)}
	$$\int\frac{\d{dt}}{3\sin x+ 4\cos x + 10} = \begin{bmatrix}
		t =\tg{\frac x2}\\
		\sin x = \frac{2t}{1+t^2} \\
		\cos x = \frac{1-t^2}{1+t^2}\\
		\dx = \frac{2}{1+t^2}\d{dt}
	\end{bmatrix} = \int \frac{\d{dt}}{\frac{6t}{1+t^2}+\frac{4-4t^2}{1+t^2} + 10} \frac{2}{1+t^2} =$$ $$ \int\frac{1}{3t^2+3t+7}\d{dt} = \frac{1}{\sqrt{19/4}}\cdot \arctg{\frac{t+3/2}{\sqrt{19/4}}} + C$$
	\subsection*{e)}
	$$\int \frac{1-\sqrt{x^2+x+1}}{x\sqrt{x^2+x+1}}\begin{bmatrix} \sqrt{x^2+x+1} = xt+1 \\
		\dx = \frac{2t^2-2t+2}{(1-t^2)^2} \\
		x = \frac{2t-1}{1-t^2}
	\end{bmatrix} = -2\int \frac{t}{2t-1} \cdot \frac{t^2-t+1}{1-t^2}\d{dt} = 2\int\frac{t(t^2-t+1)}{(2t-1)(t^2-1)^2}\d{dt} = $$ 
	$$\int \frac{t}{(2t-1)(t^2-1)}\d{dt} = \int -\frac{1}{6t+6} - \frac{2}{3(t-1)} + \frac{1}{2(t+1)} = -\frac16\ln(|t+1|) - \frac23\ln{|t-1|} + \frac12\ln{|t+1|}+C$$
\end{document}