\input{preambula.tex}
\newcommand{\ac}{\frac{a+c}{2}}
\newcommand{\bc}{\frac{b+c}{2}}
\newcommand{\ab}{\frac{a+b}{2}}
\begin{document}
	\section*{1}
	$$\left(123456789, 987654321\right) = \left(123456789, 864197532\right)  = \left(123456789, 740740743\right)  = \left(123456789, 617283954\right) $$ 
	$$\left(123456789, 493827165\right) =  \left(123456789, 370370376\right) = \left(123456789, 246913587\right) = \left(123456789, 123456798\right)$$ 
	$$ = \left(123456789, 9\right) = 9(9|123456798)$$
	\section*{2}
	\subsection*{a)}
	$$\frac{2n+13}{n+7}$$ 
	$$\left(2n+13,n+7\right) = \left(n+6,n+7\right) = \left(n+6,1\right) = 1 \to  \text{Дробь несократима}$$
	\subsection*{б)}
	$$\frac{2n^2-1}{n+1}$$
	$$\left(2n^2-1, n+1\right) = (2n^2-1, 2n^2-2) = (2n^2-1,1) = 1 \to \text{Дробь несократима}$$
	\section*{3}
		$$\left(\bc, \ac,\ab\right) = \left(\bc+\ab-\ac, \ac+\ab-\bc, \ac+\bc-\ab \right) = $$ $$=\left(a,b,c \right)$$ 
	\section*{4}
	$$\frac{C_a^b}{a}= \frac{(a-b+1)(a-b+2)\cdots(a-1)}{b!} \blacksquare$$
	\section*{5}
	Пусть n>m
	$$(f_n,f_m) = (2^{2^n}+1,2^{2^m}+1) = (2^{2^n}-2^{2^m}, 2^{2^m}+1) = 1. $$
	$$2^{2^n}-2^{2^m}-\text{делится на степень двойки, а второе число нечетное.}$$
\end{document}